Prove correctness of BernoulliExpNeg for γ > 1 (#121)
By submitting this pull request, I confirm that my contribution is made
under the terms of the [MIT
license](https://github.com/dafny-lang/dafny/blob/master/LICENSE.txt).

src/Distributions/BernoulliExpNeg/Model.dfy
@@ -18,9 +18,9 @@ module BernoulliExpNeg.Model {
     decreases gamma.numer
   {
     if gamma.numer <= gamma.denom
-    then SampleGammaLe1(gamma)
+    then SampleLe1(gamma)
     else Monad.Bind(
-        SampleGammaLe1(Rationals.Int(1)),
+        SampleLe1(Rationals.Int(1)),
         b =>
           var res: Monad.Hurd<bool> :=
             if b
@@ -30,30 +30,30 @@ module BernoulliExpNeg.Model {
       )
   }
 
-  ghost function SampleGammaLe1(gamma: Rationals.Rational): Monad.Hurd<bool>
+  ghost function SampleLe1(gamma: Rationals.Rational): Monad.Hurd<bool>
     requires 0 <= gamma.numer <= gamma.denom
   {
     Monad.Bind(
-      GammaLe1Loop(gamma)((true, 0)),
+      Le1Loop(gamma)((true, 0)),
       (ak: (bool, nat)) => Monad.Return(ak.1 % 2 == 1)
     )
   }
 
-  opaque ghost function GammaLe1Loop(gamma: Rationals.Rational): ((bool, nat)) -> Monad.Hurd<(bool, nat)>
+  opaque ghost function Le1Loop(gamma: Rationals.Rational): ((bool, nat)) -> Monad.Hurd<(bool, nat)>
     requires 0 <= gamma.numer <= gamma.denom
   {
-    GammaLe1LoopTerminatesAlmostSurely(gamma);
+    Le1LoopTerminatesAlmostSurely(gamma);
     Loops.While(
-      GammaLe1LoopCondition,
-      GammaLe1LoopIter(gamma)
+      Le1LoopCondition,
+      Le1LoopIter(gamma)
     )
   }
 
-  ghost function GammaLe1LoopCondition(ak: (bool, nat)): bool {
+  ghost function Le1LoopCondition(ak: (bool, nat)): bool {
     ak.0
   }
 
-  ghost function GammaLe1LoopIter(gamma: Rationals.Rational): ((bool, nat)) -> Monad.Hurd<(bool, nat)>
+  ghost function Le1LoopIter(gamma: Rationals.Rational): ((bool, nat)) -> Monad.Hurd<(bool, nat)>
     requires 0 <= gamma.numer <= gamma.denom
   {
     (ak: (bool, nat)) =>
@@ -67,9 +67,9 @@ module BernoulliExpNeg.Model {
     a => Monad.Return((a, k))
   }
 
-  lemma {:axiom} GammaLe1LoopTerminatesAlmostSurely(gamma: Rationals.Rational)
+  lemma {:axiom} Le1LoopTerminatesAlmostSurely(gamma: Rationals.Rational)
     requires 0 <= gamma.numer <= gamma.denom
-    ensures Loops.WhileTerminatesAlmostSurely(GammaLe1LoopCondition, GammaLe1LoopIter(gamma))
+    ensures Loops.WhileTerminatesAlmostSurely(Le1LoopCondition, Le1LoopIter(gamma))
 
 
 }
